need to rework plugin commands

theories/loader.v
@@ -1,2 +1,60 @@
 Set Debug "backtrace".
 Declare ML Module "coq-mebi.mebi".
+
+Inductive output_mode : Set :=
+| RunCheck : output_mode (* only warning printouts *)
+| ShowInfo : output_mode (* show more printouts *)
+| Verbose  : output_mode (* show more detailed printouts *)
+.
+Definition DefaultOutputMode := RunCheck.
+
+Inductive plugin_model_kind : Set :=
+| AsLTS : plugin_model_kind
+| AsFSM : plugin_model_kind
+.
+Definition DefaultPluginModelKind := AsLTS.
+
+Section Definitions.
+  Context (M : Type) (A : Type).
+  Definition LTS : Type := M -> option A -> M -> Prop.
+  Inductive term_to_model : Type := ModelInfo : A -> LTS -> term_to_model.
+End Definitions.
+About ModelInfo.
+Arguments term_to_model {M A}.
+
+(* Section ModelCommands.
+  Context (M : Type) (A : Type).
+  Inductive plugin_model_params : Type := 
+  | Model : plugin_model_kind -> option nat -> term_to_model -> plugin_model_params
+.
+Definition DefaultPluginModel := Model DefaultPluginModelKind None.
+
+Inductive dev_plugin_command : Type :=
+| Saturate : plugin_model_params -> dev_plugin_command
+.
+
+Inductive plugin_command : Type :=
+| Bisim : plugin_model_params -> plugin_model_params
+
+
+End API. *)
+
+
+
+
+(* Definition  *)
+(* Record coq_lts := { term_type  : A; label_type : B }. *)
+
+(* Definition term {A B : Type} :=  *)
+
+(* Inductive build_model {A B : Type} (p:A) (ls:list coq_lts) := *)
+(* | *)
+
+(* Inductive build_model (A:Type) (B:Type) (a:A) (l:(A -> option B -> A -> Prop)) : Type :=
+| LTS : build_model A B a l
+| FSM : build_model A B a l
+. *)
+
+
+(* Inductive run_mode : Set :=
+|  *)
